test/tactic/classical.lean
@@ -1,0 +1,20 @@
+
+import util.classical
+
+universes u v
+
+variables {α : Type u}
+variables {β : Type v}
+variables {p q : α → Prop}
+variables Hall : ∀ x, p x → q x
+variables Hex : ∃ x, p x
+
+lemma some_spec_test1
+: p (classical.some Hex) :=
+by { apply_some_spec with w, }
+
+include Hall
+
+lemma some_spec_test2
+: q (classical.some Hex) :=
+by { apply_some_spec with w, apply Hall w }
